blood_search

dafny/Blood.dfy
@@ -51,8 +51,100 @@ class Blood {
             result := false;
         }
     }
+    /*
+test_state:
+1 = not tested (directly comes from Bat-mobile)
+2 = Good blood
+3 = Bad blood
+
+state:
+1 = in inventory
+2 = testing (in pathologies)
+3 = used (by organization)
+4 = disposed (expired blood and disposed by vampire)
+*/
+
+class Blood {
+    var add_time: int;
+    var use_by: int; // UTC seconds since 1970-01-01 00:00:00 GTM
+    var state: int;
+    var test_state: int;
+    var blood_type: string;
+    var id: int;
+    predicate valid()
+    reads this
+    {
+        add_time >= 0 && use_by >= 0 && state >= 1 && state <= 4
+    &&  test_state >=1 && test_state <= 3 && blood_type != ""
+    }
+
+    constructor(){
+
+    }    
+
+    // constructor(add_time:int , use_by:int,state : int , test_state:int , blood_type:string) 
+    // modifies this;
+    // {
+    //     this.add_time := add_time;
+    //     this.use_by := use_by;
+    //     this.state := state;
+    //     this.test_state := test_state;
+    //     this.blood_type := blood_type;
+    // }
+
+    // should be moved to some upper level methods
+    method is_expired(curr_time: int) returns (expired: bool)
+    // requires curr_time is correct, but we cannot prove this
+    requires valid();
+    ensures valid();
+    ensures expired <==> use_by >= curr_time;
+    {
+        if (curr_time > use_by){
+            expired := false;
+        }
+        else {
+            expired := true;
+        }
+    }
+
+    method blood_test(test_state:int) 
+    requires test_state>=1 && test_state<=3;
+    requires valid();
+    ensures valid();
+    modifies this;
+    {
+        this.test_state := test_state;
+    }
+    
+    method is_good_blood() returns (result: bool)
+    requires valid();
+    ensures valid();
+    ensures result == (test_state == 2)
+    {
+        if(test_state == 2){
+            result := true;
+        } else{
+            result := false;
+        }
+    }
+    method search_blood_by_id(a:array<Blood>,key:int) returns(res:int)
+    ensures res!=-1 ==> (0<=res<a.Length && a[res].id==key)
+    ensures res==-1 ==> forall k:: 0<=k<a.Length ==> a[k].id!=key
+    {
+        res:=0;
+        while res<a.Length
+        invariant 0<=res<=a.Length
+        invariant forall k:: 0<=k<res ==> a[k].id!=key
+        decreases a.Length-res
+        {
+            if(a[res].id==key){
+                return res;
+            }
+            res:=res+1;
+        }
+        res:=-1;
+        
+    }
 }
-
-
 
 
